assembler/RelocProgLinking.v
@@ -1,0 +1,15 @@
+Require Import Coqlib Integers Values Maps AST.
+Require Import RelocProg.
+Require Import Linking Errors.
+Import ListNotations.
+
+Local Open Scope list_scope.
+
+Definition link_reloc_prog (F V I D: Type) (p1 p2: program F V I D) : option (program F V I D) := None.
+
+Program Instance Linker_reloc_prog (F V I D : Type) : Linker (program F V I D) :=
+{
+  link := (link_reloc_prog F V I D);
+  linkorder := fun _ _ => True;
+}.
+
