elf/RelocElfLinking.v
@@ -1,0 +1,15 @@
+Require Import Coqlib Integers Values Maps AST.
+Require Import RelocElf.
+Require Import Linking Errors.
+Import ListNotations.
+
+Local Open Scope list_scope.
+
+Definition link_elf_file (p1 p2: elf_file) : option elf_file := None.
+
+Program Instance Linker_elf_file : Linker elf_file :=
+{
+  link := link_elf_file;
+  linkorder := fun _ _ => True;
+}.
+
